LeanBF/Theory/Simulate.lean
@@ -4,20 +4,12 @@ Released under Apache 2.0 license as described in the file LICENSE.
 Authors: Bangyen Pham
 -/
 
-import LeanBF.Theory.Simulate.Basics
-import LeanBF.Theory.Simulate.CompileBody
 import LeanBF.Theory.Simulate.CompileInstr
-import LeanBF.Theory.Simulate.CompileInstrJzdec1
-import LeanBF.Theory.Simulate.CompileInstrJzdec2
-import LeanBF.Theory.Simulate.CompileProgram
-import LeanBF.Theory.Simulate.DispatchLemmas
-import LeanBF.Theory.Simulate.DispatchStep
-import LeanBF.Theory.Simulate.JzdecThenElse
-import LeanBF.Theory.Simulate.WindowDone
-import LeanBF.Theory.Simulate.WindowInc
-import LeanBF.Theory.Simulate.WindowJzdecHalt
-import LeanBF.Theory.Simulate.WindowMatch
-import LeanBF.Theory.Simulate.WindowSkip
+import LeanBF.Theory.Simulate.CompileInstrJzdec
+import LeanBF.Theory.Simulate.CompileLoop
+import LeanBF.Theory.Simulate.Dispatch
+import LeanBF.Theory.Simulate.WindowInstr
+import LeanBF.Theory.Simulate.WindowMatchSkip
 
 /-!
 # Dispatch Simulation Aggregator
